vcg/VCG_Search_as_General_VCG.v
@@ -31,6 +31,7 @@
 *)
  
 From Coq Require Import Unicode.Utf8.
+From HB Require Import structures.
 From mathcomp Require Import all_ssreflect order.
 From mathcomp.fingroup Require Import perm.
 
@@ -77,16 +78,13 @@ Definition slot_succ (s : slot) : slot := ord_succ s.
 
 Definition last_slot : slot := ord_max.
 
-Definition slot_as_agent (s : slot) : A.
-have slot_as_agent_p : s < n by exact: leq_trans (ltn_ord s) le_k_n.
-exact: (Ordinal slot_as_agent_p).
-Defined.
+Definition slot_as_agent (s : slot) : A := widen_ord le_k_n s.
 
 Lemma slot_as_agent_inj : injective slot_as_agent.
 Proof.
-move=> s1 s2 /eqP.
-rewrite /slot_as_agent /sval -(inj_eq val_inj) /= => /eqP.
-exact: val_inj.
+move=> s1 s2 H.
+apply: val_inj.
+exact: (congr1 val H).
 Qed.
 
 End Slot.
@@ -201,13 +199,9 @@ Defined.
 
 Coercion obidders : O >-> tuple_of.
 
-Canonical O_subType := Eval hnf in [subType for obidders].
-Canonical O_eqType := Eval hnf in EqType _ [eqMixin     of O by <: ].
-Canonical O_choiceType := Eval hnf in ChoiceType _ [choiceMixin of O by <:].
-Canonical O_countType := Eval hnf in CountType _ [countMixin  of O by <:].
-Canonical O_subCountType := Eval hnf in [subCountType of O].
-Canonical O_finType := Eval hnf in FinType _ [finMixin    of O by <:].
-Canonical O_subFinType := Eval hnf in [subFinType of O].
+#[export] HB.instance Definition _ := [isSub for obidders].
+#[export] HB.instance Definition _ := [Finite of O by <:].
+Definition O_finType := [the finType of O].
 
 Set Warnings "-projection-no-head-constant".
 Canonical O_predType := PredType (fun o x => x \in obidders o).
@@ -753,7 +747,7 @@ Lemma bidsSum_sumBid (P : A -> bool) (o : O) :
   forall bs, \sum_(j < n | P j) tnth (biddings bs) j o = \sum_(j < n | P j) bidding bs j o.
 Proof. by move=> ?; apply: congr_big => //= j _; rewrite tnth_mktuple. Qed.
 
-Definition max_bidSum_spec := (@extremum_spec [eqType of nat] geq O_finType predT bidSum).
+Definition max_bidSum_spec := (@extremum_spec nat geq O_finType predT bidSum).
 
 Lemma VCG_oStar_extremum : max_bidSum_spec VCG_oStar.
 Proof. exact: arg_maxnP. Qed.
@@ -837,7 +831,7 @@ Qed.
 
 Lemma lt_bidSum_out (o1 o2 : O) s  
   (l21 : 'bid_ (tnth o2 s) < 'bid_ (tnth o1 s)) 
-  (out2 : ∀ x : ordinal_finType k, tnth o2 x != tnth o1 s) : 
+  (out2 : ∀ x : 'I_k, tnth o2 x != tnth o1 s) : 
   let o2' :=  Outcome (uniq_set_o s out2) in
   'ctr_ s != ctr0 -> bidSum o2 < bidSum o2'.
 Proof.
@@ -1377,7 +1371,7 @@ rewrite bidsSum_sumBid -valid_bidSum bidSum_slot.
 apply: eq_bigr => j _.
 rewrite /bidding ffunE /bidding /t_bidding /bid_ctr_slot !tnth_map !tnth_ord_tuple.
 - have [] := boolP (widen_ord le_k_n j \in oStar_i) => jin.  
-  congr ('bid_ _ * 'ctr_ _); first by exact: widen_slot_as_agent.
+  congr ('bid_ _ * 'ctr_ _); first by [].
   rewrite (@slot_in_oStar bs0) //.
   apply: val_inj => /=.
   by rewrite inordK.
@@ -1390,7 +1384,7 @@ Qed.
 (** Price equality, when agent [i] loses. *)
 
 Lemma eq_sorted_VCG_price_loses :  
-  price bs i = @G.price [finType of O] o0 i (biddings bs).
+  price bs i = @G.price [the finType of O] o0 i (biddings bs).
 Proof.
 rewrite /price /is_winner tsortK ?idxaK // /price /externality G.eq_price'' /G.price''.
 rewrite -/welfare_without_i'' -/welfare_with_i.
@@ -1868,7 +1862,7 @@ Qed.
 (** Price equality, when agent [i] wins. *)
 
 Lemma eq_sorted_VCG_price_wins :  
-  price bs i = @G.price [finType of O] o0 i (biddings bs).
+  price bs i = @G.price [the finType of O] o0 i (biddings bs).
 Proof.
 rewrite /price /is_winner tsortK ?idxaK //. 
 rewrite /price /is_winner /externality G.eq_price'' /G.price''.
@@ -1932,7 +1926,7 @@ Qed.
 End Wins.
 
 Lemma eq_sorted_VCG_price :
-  price bs i = @G.price [finType of O] o0 i (biddings bs).
+  price bs i = @G.price [the finType of O] o0 i (biddings bs).
 Proof.
 have [] := boolP (i < k) => iisslot; 
   first by rewrite eq_sorted_VCG_price_wins // (mem_oStar sorted_bs0).
@@ -1994,8 +1988,8 @@ rewrite !tnth_mktuple.
 by apply/ffunP => o'; rewrite -relabelled_bidding permE -{1}(cancel_inv_idxa bs j).
 Qed.  
 
-Definition instance_vcg_price := @G.price [finType of O] o0 i (instance_biddings bs).
-Definition instance_vcg_price' := @G.price [finType of O] o0 i' (instance_biddings bs').
+Definition instance_vcg_price := @G.price [the finType of O] o0 i (instance_biddings bs).
+Definition instance_vcg_price' := @G.price [the finType of O] o0 i' (instance_biddings bs').
 
 Lemma eq_instance_vcg_price : instance_vcg_price' = instance_vcg_price.
 Proof. 
